Remove redundant get_jump_offset calc. from line_ok
Progress on #107

compiler/backend/lab_to_targetScript.sml
@@ -181,32 +181,27 @@ val line_length_def = Define `
   (line_length (LabAsm a w bytes l) = LENGTH bytes)`
 
 val line_ok_light_def = Define `
-  (line_ok_light (c:'a asm_config) labs pos (Label _ _ l) <=> T) /\
-  (line_ok_light c labs pos (Asm b bytes l) <=> asm_ok b c) /\
-  (line_ok_light c labs pos (LabAsm Halt w bytes l) <=>
-     let w1 = (0w:'a word) - n2w (pos + ffi_offset) in
-        asm_ok (Jump w1) c) /\
-  (line_ok_light c labs pos (LabAsm ClearCache w bytes l) <=>
-     let w1 = (0w:'a word) - n2w (pos + 2 * ffi_offset) in
-        asm_ok (Jump w1) c) /\
-  (line_ok_light c labs pos (LabAsm (CallFFI index) w bytes l) <=>
-     let w1 = (0w:'a word) - n2w (pos + (3 + index) * ffi_offset) in
-        asm_ok (Jump w1) c) /\
-  (line_ok_light c labs pos (LabAsm (Call v24) w bytes l) <=>
+  (line_ok_light (c:'a asm_config) labs (Label _ _ l) <=> T) /\
+  (line_ok_light c labs (Asm b bytes l) <=> asm_ok b c) /\
+  (line_ok_light c labs (LabAsm Halt w bytes l) <=>
+     asm_ok (Jump w) c) /\
+  (line_ok_light c labs (LabAsm ClearCache w bytes l) <=>
+     asm_ok (Jump w) c) /\
+  (line_ok_light c labs (LabAsm (CallFFI index) w bytes l) <=>
+     asm_ok (Jump w) c) /\
+  (line_ok_light c labs (LabAsm (Call v24) w bytes l) <=>
      F (* Call not yet supported *)) /\
-  (line_ok_light c labs pos (LabAsm a w bytes l) <=>
-     let target = find_pos (get_label a) labs in
-     let w1 = n2w target - n2w pos in
-        asm_ok (lab_inst w1 a) c /\
-       (case get_label a of Lab l1 l2 => (lab_lookup l1 l2 labs <> NONE)))`
+  (line_ok_light c labs (LabAsm a w bytes l) <=>
+     asm_ok (lab_inst w a) c /\
+     (case get_label a of Lab l1 l2 => (lab_lookup l1 l2 labs <> NONE)))`
 
-val all_enc_ok_light_def = Define `
-  (all_enc_ok_light c labs pos [] = T) /\
-  (all_enc_ok_light c labs pos ((Section k [])::xs) <=>
-     all_enc_ok_light c labs pos xs) /\
-  (all_enc_ok_light c labs pos ((Section k (y::ys))::xs) <=>
-     line_ok_light c labs pos y /\
-     all_enc_ok_light c labs (pos + line_length y) ((Section k ys)::xs))`
+val sec_ok_light_def = Define`
+  sec_ok_light c labs (Section k ls) ⇔
+    EVERY (line_ok_light c labs) ls`;
+val _ = export_rewrites["sec_ok_light_def"];
+
+val _ = overload_on("all_enc_ok_light",``λc labs ls.
+  EVERY (sec_ok_light c labs) ls``);
 
 (* pad with nop byte, and nop instruction *)
 
@@ -294,7 +289,7 @@ val remove_labels_loop_def = Define `
         (* move label padding into instructions *)
         let sec_list = pad_code (c.encode (Inst Skip)) sec_list in
         (* it ought to be impossible for done to be false here *)
-          if done /\ all_enc_ok_light c labs 0 sec_list
+          if done /\ all_enc_ok_light c labs sec_list
           then SOME (sec_list,labs)
           else NONE
       else
